\section*{Problem 2}
\noindent
Proving the Geometric Series Identity\\
Let $\displaystyle S_n=a^0+a^1+a^2+\cdots+a^{n-1}$\\
$\displaystyle aS_n=a^1+a^2+a^3+\cdots+a^{n}$\\
$\displaystyle aS_n-S_n=a^1+a^2+\cdots+a^{n}-(a^0+a^1+\cdots a^{n-1})$\\
$\displaystyle S_n(a-1)=a^{n}-a^0$\\
$\displaystyle S_n=\frac{a^{n}-1}{a-1},a\neq1$

\begin{center}
\rule{\textwidth}{.1pt}
\end{center}

\noindent
Let $\displaystyle S_n=0+\frac{1}{4}+\frac{2}{4^2}+\cdots+\frac{n-1}{4^{n-1}}$\\
$\displaystyle 4S_n=\frac{1}{4^0}+\frac{2}{4^2}+\cdots+\frac{n-1}{4^{n-2}}$\\
$\displaystyle 4S_n-S_n=\frac{1}{4^0}+\frac{2}{4^1}-\frac{1}{4^1}+\frac{3}{4^2}-\frac{2}{4^2}+\cdots+\frac{n-1}{4^{n-1}}-\frac{n-2}{4^{n-1}}$\\
$\displaystyle 3S_n=\frac{1}{4^0}+\frac{1}{4^2}+\frac{1}{4^3}+\cdots+\frac{1}{4^{n-1}}$\\
$\displaystyle 3S_n=\sum_{k=0}^{n}\frac{1}{4^k}$

\begin{center}
\rule{\textwidth}{.1pt}
\end{center}

\noindent
Evaluate $\displaystyle\sum_{k=0}^{\infty}\frac{1}{4^k}$
\begin{align*}
\sum_{k=0}^{\infty}\frac{1}{4^k} &= \lim_{k\to\infty}\frac{\left(\frac{1}{4}\right)^n-1}{-\frac{3}{4}}      \\
                                 &= \lim_{k\to\infty}-\frac{4}{3}\left[\left(\frac{1}{4}\right)^n-1\right]  \\
                                 &= -\frac{4}{3}\lim_{k\to\infty}\left[\left(\frac{1}{4}\right)^k-1\right]  \\
                                 &= \frac{4}{3}
\end{align*}

\begin{center}
\rule{\textwidth}{.1pt}
\end{center}
\clearpage

\noindent
Substitute this value back into the original series\\
$\displaystyle 3S_n=\sum_{k=0}^{n}\frac{1}{4^k}$\\
$\displaystyle 3S_{\infty}=\sum_{k=0}^{\infty}\frac{1}{4^k}$\\
$\displaystyle 3S_{\infty}=\frac{4}{3}$\\
$\displaystyle S_{\infty}=\frac{4}{9}$

\[
    \sum_{i=0}^{\infty}\frac{i}{4^i}=\frac{4}{9}
\]

\begin{center}
\rule{\textwidth}{3pt}
\end{center}
