\clearpage
\section*{Problem 1}
\begin{enumerate}[A.]
    \item Prove that $\displaystyle\log_{c}(ab)=\log_{c}a+\log_{c}b$
    
    Let $x=\log_{c}a$, $y=\log_{c}b$\\
    Using the definition of the logarithm, $c^x=a$,$c^y=b$.\\
    $ab=c^x\cdot c^y$\\
    $ab=c^{x+y}$\\
    $\log_c{ab}=x+y$
    
    Substituting back for $x$ and $y$,\\
    $\log_c{ab}=\log_{c}a+\log_{c}b$\\
    $\square$
    
    \item Prove that $\displaystyle\log_{c}(a^{b})=b\log_{c}a$
    
    Let $x=\log_{c}(a)$\\
    Using the definition of the logarithm, $c^x=a$
    
    Substituting for $a$:\\
    $\log_{c}(a^{b})=\log_{c}((c^{x})^{b})$\\
    $=\log_{c}(c^{xb})$\\
    $=xb$
    
    Substituting $x$ back for its definition\\
    $xb=b\log_{c}(a)$\\
    $\therefore\log_{c}(a^{b})=b\log_{c}(a)$\\
    $\square$
    
    \item Prove that $\displaystyle\log_{b}a=\frac{\log_{c}a}{\log_{c}b}$
    
    Let $x=\log_{b}(a)$\\
    Using the definition of the logarithm, $b^{x}=a$\\
    Taking a logarithm to both sides $\log_{c}(b^{x})=\log_{c}a$
    
    Using the product rule, $x\log_{c}b=\log_{c}a$\\
    $\displaystyle x=\frac{\log_{c}a}{\log_{c}b}$
    
    Substituting $x$ for its definition,\\
    $\displaystyle\log_{b}a=\frac{\log_{c}a}{\log_{c}b}$\\
    $\square$
    
\end{enumerate}